toy code example to extract to C

examples/low-level/ulib/ml/FStar_SST.ml
@@ -1,0 +1,5 @@
+let push_frame () = ()
+let pop_frame () = ()
+let salloc a = ref a
+let op_Bang a = !a
+let get () = ()
