examples/low-level/ulib/ml/SInt_UInt8.ml
@@ -1,0 +1,69 @@
+open Char
+
+let n = 8
+
+type uint8 = int
+
+let (zero:uint8) = 0
+let (one:uint8) = 1
+let (ones:uint8) = 255
+
+let bits = 8
+
+(* Standard operators *)
+let add a b = ((a + b) land 255)
+let add_mod a b =  (( a +  b) land 255)
+let sub a b = (( a -  b) land 255)
+let sub_mod a b =  (( a -  b) land 255)
+let mul a b =  (( a *  b) land 255)
+let mul_mod a b =  (( a *  b) land 255)
+let div a b =  (( a /  b) land 255)
+let rem a b =  ( a mod  b)
+
+let logand a b =  ( a land  b)
+let logxor a b =  ( a lxor  b)
+let logor a b =  ( a lor  b)
+let lognot a =  (lnot ( a land 255))
+
+let shift_left a s = a lsl s
+let shift_right a s = a lsr s
+
+let rotate_left a s =  ((( a lsl s) + ( a lsr (8-s))) land 255)
+let rotate_right a s =  ((( a lsl (8-s)) + ( a lsr s)) land 255)
+
+let gte x y = (lnot((x - y) asr 7)) land 255
+
+(* let eq a b = *)
+(*   let a = lnot(a lxor b) in *)
+(*   let a = a land (a lsl 32) in *)
+(*   let a = a land (a lsl 16) in *)
+(*   let a = a land (a lsl 8) in *)
+(*   let a = a land (a lsl 8) in *)
+(*   let a = a land (a lsl 4) in *)
+(*   let a = a land (a lsl 2) in *)
+(*   let a = a land (a lsl 1) in *)
+(*   (a asr 62) land 255 *)
+
+let eq x y = gte x y land gte y x
+                                           
+let op_Hat_Plus = add
+let op_Hat_Subtraction = sub
+let op_Hat_Star = mul
+let op_Hat_Slash = div
+let op_Hat_Plus_Percent = add_mod
+let op_Hat_Star_Percent = mul_mod
+let op_Hat_Subtraction_Percent = sub_mod
+let op_Hat_Less_Less  = shift_left
+let op_Hat_Greater_Greater  = shift_right
+let op_Hat_Amp = logand
+let op_Hat_Hat = logxor
+let op_Hat_Bar = logor
+
+let of_string s =
+  let x = int_of_string s in
+  if x >= 256 || x < 0 then failwith "Wrong constant"
+  else x 
+let of_int s = s land 255
+                                                             
+let to_string s = string_of_int s
+let to_int s = s
