examples/low-level/ulib/SInt.UInt8.fst
@@ -1,0 +1,82 @@
+module SInt.UInt8
+
+(* Defines secret bytes *)
+
+open FStar.Ghost
+open Axioms
+open IntLib
+open SInt
+
+let n = 8 
+
+type uint8 = usint n
+type sbyte = uint8
+
+let (zero:uint8) = uzero n
+let (one:uint8) = uone n
+let (ones:uint8) = uones n
+
+let (max_int:erased nat) = eumax_int #n
+let (min_int:erased nat) = eumin_int #n
+
+let (bits:pos) = n
+
+(* Standard operators *)
+val add: a:uint8 -> b:uint8{v a + v b < pow2 n} -> Tot uint8
+val add_mod: a:uint8 -> b:uint8 -> Tot uint8
+val sub: a:uint8 -> b:uint8{v a - v b >= 0} -> Tot uint8
+val sub_mod: a:uint8 -> b:uint8 -> Tot uint8
+val mul: a:uint8 -> b:uint8{v a * v b < pow2 n} -> Tot uint8
+val mul_mod: a:uint8 -> b:uint8 -> Tot uint8
+val div: a:uint8 -> b:uint8{v b <> 0} -> Tot uint8
+val rem: a:uint8 -> b:uint8{v b <> 0} -> Tot uint8
+val logand: uint8 -> uint8 -> Tot uint8
+val logxor: uint8 -> uint8 -> Tot uint8
+val logor: uint8 -> uint8 -> Tot uint8
+val lognot: uint8 -> Tot uint8
+val shift_right: a:uint8 -> s:nat -> Tot uint8
+val shift_left: a:uint8 -> s:nat -> Tot uint8
+val rotate_left: a:uint8 -> s:nat{s <= n} -> Tot uint8
+val rotate_right: a:uint8 -> s:nat{s <= n} -> Tot uint8
+let add a b = uadd #n a b
+let add_mod a b = uadd_mod #n a b
+let sub a b = usub #n a b
+let sub_mod a b = usub_mod #n a b
+let mul a b = umul #n a b
+let mul_mod a b = umul_mod #n a b
+let div a b = udiv #n a b
+let rem a b = umod #n a b
+let logand a b = ulogand #n a b
+let logxor a b = ulogxor #n a b
+let logor a b = ulogor #n a b
+let lognot a = ulognot #n a
+let shift_left a s = ushift_left #n a s
+let shift_right a s = ushift_right #n a s
+let rotate_left a s = urotate_left #n a s
+let rotate_right a s = urotate_right #n a s
+
+let to_uint8 s = to_usint n s
+let of_native_int s = to_usint n s
+
+assume val of_string: string -> Tot uint8
+assume val of_int: x:nat{x >= 0 /\ x < pow2 n} -> Tot (y:uint8{v y = x})
+
+let op_Hat_Plus = add
+let op_Hat_Plus_Percent = add_mod
+let op_Hat_Star = mul
+let op_Hat_Star_Percent = mul_mod
+let op_Hat_Slash = div
+let op_Hat_Subtraction = sub 
+let op_Hat_Subtraction_Percent = sub_mod
+let op_Hat_Less_Less  = shift_left 
+let op_Hat_Greater_Greater  = shift_right 
+let op_Less_Less_Less = rotate_left
+let op_Greater_Greater_Greater = rotate_right
+let op_Hat_Amp = logand
+let op_Hat_Hat = logxor
+let op_Hat_Bar = logor
+
+assume val eq: x:uint8 -> y:uint8 -> Tot (z:uint8{(v x = v y <==> v z = pow2 8 - 1)
+								  /\ (v x <> v y <==> v z = 0)})
+assume val gte: x:uint8 -> y:uint8 -> Tot (z:uint8{(v x >= v y <==> v z = pow2 8 - 1)
+								  /\ (v x < v y <==> v z = 0)})
