examples/low-level/ulib/SInt.fst
@@ -1,0 +1,195 @@
+module SInt
+open Axioms
+open FStar.Ghost
+open IntLib
+ 
+(** Opaque integers **)
+assume new type sint : Type0
+
+(* Mathematical ghost value of the sint *)
+assume val v: x:sint -> GTot int
+let ssize (x:sint) (n:pos) : GTot Type0 = (v x >= -(pow2 (n-1)) /\ v x < pow2 (n-1))
+let usize (x:sint) (n:nat)   : GTot Type0 = (v x >= 0 /\ v x < pow2 n)
+
+(* Concrete types *)
+type ssint (n:pos) = x:sint{ssize x n}
+type usint (n:nat) = x:sint{usize x n}
+
+(* Specs *)
+assume val esmax_int: #n:pos -> Tot (max:erased nat{reveal max = pow2 (n-1) - 1})
+assume val eumax_int: #n:nat -> Tot (max:erased nat{reveal max = pow2 n - 1})
+assume val smax_int: #n:pos -> GTot (max:nat{max = pow2 (n-1) - 1})
+assume val umax_int: #n:nat -> GTot (max:nat{max = pow2 n - 1})
+
+assume val esmin_int: #n:pos -> Tot (min:erased nat{reveal min = - (pow2 (n-1))})
+assume val eumin_int: #n:nat -> Tot (min:erased nat{reveal min = 0})
+assume val smin_int: #n:pos -> GTot (min:nat{min = - (pow2 (n-1))})
+assume val umin_int: #n:nat -> GTot (min:nat{min = 0})
+
+(* Zero for signed and unsiged words *)
+assume val szero: n:pos -> Tot (z:ssint n{v z = 0})
+assume val uzero: n:nat -> Tot (z:usint n{v z = 0})
+(* One for signed and unsigned words *)
+assume val sone: n:pos{n > 1} -> Tot (o:ssint n{v o = 1})
+assume val uone: n:pos -> Tot (o:usint n{v o = 1})
+(* All ones mask for signed and unsigned words *)
+assume val sones: n:pos{n > 1} -> Tot (o:ssint n{v o = -1})
+assume val uones: n:pos -> Tot (o:usint n{v o = pow2 n - 1})
+
+(* Increment and decrement *)
+assume val sincr: #n:pos -> a:ssint n{v a < smax_int #n} -> Tot (b:ssint n{v b = v a + 1})
+assume val uincr: #n:pos -> a:usint n{v a < umax_int #n} -> Tot (b:usint n{v b = v a + 1})
+assume val spred: #n:pos -> a:ssint n{v a > smin_int #n} -> Tot (b:ssint n{v b = v a - 1})
+assume val upred: #n:pos -> a:usint n{v a > umin_int #n} -> Tot (b:usint n{v b = v a - 1})
+
+assume val sincr_mod: #n:pos -> a:ssint n -> Tot (b:ssint n{v b = cmod (v a + 1) (pow2 n)})
+assume val uincr_mod: #n:pos -> a:usint n -> Tot (b:usint n{v b = (v a + 1) % (pow2 n)})
+assume val spred_mod: #n:pos -> a:ssint n -> Tot (b:ssint n{v b = cmod (v a - 1) (pow2 n)})
+assume val upred_mod: #n:pos -> a:usint n -> Tot (b:usint n{v b = (v a - 1) % (pow2 n)})
+
+(* Addition primitives *)
+assume val sadd: #n:pos -> a:ssint n ->
+  b:ssint n{v a + v b < pow2 (n-1) /\ v a + v b >= - (pow2 (n-1))} ->
+  Tot (c:ssint n{v c = v a + v b})
+assume val sadd_mod: #n:pos -> a:ssint n -> b:ssint n ->
+  Tot (c:ssint n{v c = cmod (v a + v b) (pow2 n)})
+assume val uadd: #n:nat -> a:usint n -> b:usint n{v a + v b < pow2 n} ->
+  Tot (c:usint n{v c = v a + v b})
+assume val uadd_mod: #n:nat -> a:usint n -> b:usint n ->
+  Tot (c:usint n{v c = (v a + v b) % (pow2 n)})
+
+(* Subtraction primitives *)
+assume val ssub: #n:pos -> a:ssint n ->
+  b:ssint n{v a - v b >= - (pow2 (n-1)) /\ v a - v b < pow2 (n-1)} ->
+  Tot (c:ssint n{v c = v a + v b})
+assume val ssub_mod: #n:pos -> a:ssint n -> b:ssint n ->
+  Tot (c:ssint n{v c = cmod (v a - v b) (pow2 n)})
+assume val usub: #n:nat -> a:usint n -> b:usint n{v a - v b >= 0} ->
+  Tot (c:usint n{v c = v a - v b})
+assume val usub_mod: #n:nat -> a:usint n -> b:usint n ->
+  Tot (c:usint n{v c = (v a - v b) % (pow2 n)})
+
+(* Multiplication primitives *)
+assume val smul: #n:pos -> a:ssint n ->
+  b:ssint n{v a * v b < pow2 (n-1) /\ v a * v b >= - (pow2 (n-1))} ->
+  Tot (c:ssint n{v c = v a * v b})
+assume val smul_mod: #n:pos -> a:ssint n -> b:ssint n ->
+  Tot (c:ssint n{v c = cmod (v a * v b) (pow2 n)})
+assume val smul_large: #n:pos -> a:ssint n -> b:ssint n ->
+  Tot (c:ssint (2*n){v c = v a * v b})
+assume val umul: #n:nat -> a:usint n -> b:usint n{v a * v b < pow2 n} ->
+  Tot (c:usint n{v c = v a * v b})
+assume val umul_mod: #n:nat -> a:usint n -> b:usint n ->
+  Tot (c:usint n{v c = (v a * v b) % (pow2 n)})
+assume val umul_large: #n:pos -> a:usint n -> b:usint n ->
+  Tot (c:usint (2*n){v c = v a * v b})
+
+(* Division primitives *)
+assume val sdiv: #n:pos -> a:ssint n ->
+  b:ssint n{v b <> 0} -> Tot (c:ssint n{v c = div (v a) (v b)})
+assume val udiv: #n:nat -> a:usint n -> b:usint n{v b <> 0} ->
+  Tot (c:usint n{v c = v a / v b})
+
+(* Modulo primitives *)
+assume val smod: #n:pos -> a:ssint n ->
+  b:ssint n{v b <> 0} -> Tot (c:ssint n{v c = div (v a) (v b)})
+assume val umod: #n:nat -> a:usint n -> b:usint n{v b <> 0} ->
+  Tot (c:usint n{v c = v a / v b})
+
+(* Negation primitives *)
+assume val sneg: #n:pos -> a:ssint n -> Tot (b:ssint n{v b = - (v a)})
+
+(* Bitwise operators *)
+assume val slogand: #n:pos -> ssint n -> ssint n -> Tot (ssint n)
+assume val slogxor: #n:pos -> ssint n -> ssint n -> Tot (ssint n)
+assume val slogor: #n:pos -> ssint n -> ssint n -> Tot (ssint n)
+assume val slognot: #n:pos -> ssint n -> Tot (ssint n)
+assume val ulogand: #n:nat -> usint n -> usint n -> Tot (usint n)
+assume val ulogxor: #n:nat -> usint n -> usint n -> Tot (usint n)
+assume val ulogor: #n:nat -> usint n -> usint n -> Tot (usint n)
+assume val ulognot: #n:nat -> usint n -> Tot (usint n)
+
+(* Bitwise operators lemmas *)
+(* TODO: add reasonable patterns *)
+(* TODO: find minimal subset *)
+(* TODO: define a 'nth' function that returns the nth bit of the sint, and prove lemmas from it *)
+assume val slogand_lemma_1: #n:pos -> a:ssint n -> b:ssint n ->
+  Lemma (requires True) (ensures (v (slogand #n a b) = v (slogand #n b a)))
+assume val slogand_lemma_2: #n:pos -> a:ssint n ->
+  Lemma (requires True) (ensures (v (slogand #n a (szero n)) = 0))
+assume val slogand_lemma_3: #n:pos{n > 1} -> a:ssint n ->
+  Lemma (requires True) (ensures (v (slogand #n a (sones n)) = v a))
+
+assume val slogxor_lemma_1: #n:pos -> a:ssint n -> b:ssint n ->
+  Lemma (requires True) (ensures (v (slogxor #n a b) = v (slogxor #n b a)))
+assume val slogxor_lemma_2: #n:pos -> a:ssint n ->
+  Lemma (requires True) (ensures (v (slogxor #n a (szero n)) = v a))
+assume val slogxor_lemma_3: #n:pos{n > 1} -> a:ssint n ->
+  Lemma (requires True) (ensures (v (slogxor #n a (sones n)) = v (slognot #n a)))
+assume val slogxor_lemma_4: n:pos -> a:ssint n ->
+  Lemma (requires True) (ensures (v (slogxor #n a a) = 0))
+
+assume val slogor_lemma_1: #n:pos -> a:ssint n -> b:ssint n ->
+  Lemma (requires True) (ensures (v (slogor #n a b) = v (slogor #n b a)))
+assume val slogor_lemma_2: #n:pos -> a:ssint n ->
+  Lemma (requires True) (ensures (v (slogor #n a (szero n)) = v a))
+assume val slogor_lemma_3: #n:pos{n > 1} -> a:ssint n ->
+  Lemma (requires True) (ensures (v (slogor #n a (sones n)) = v (sones n)))
+
+assume val slognot_lemma_1: #n:pos -> a:ssint n ->
+  Lemma (requires True) (ensures (v (slognot #n (slognot #n a)) = v a))
+assume val slognot_lemma_2: #n:pos{n > 1} ->
+  Lemma (requires True) (ensures (v (slognot #n (szero n)) = v (sones n)))
+
+assume val ulogand_lemma_1: #n:nat -> a:usint n -> b:usint n ->
+  Lemma (requires True) (ensures (v (ulogand #n a b) = v (ulogand #n b a)))
+assume val ulogand_lemma_2: #n:nat -> a:usint n ->
+  Lemma (requires True) (ensures (v (ulogand #n a (uzero n)) = 0))
+assume val ulogand_lemma_3: #n:pos -> a:usint n ->
+  Lemma (requires True) (ensures (v (ulogand #n a (uones n)) = v a))
+assume val ulogand_lemma_4: #n:nat -> a:usint n -> m:nat -> b:usint n ->
+  Lemma (requires (v b = pow2 m - 1)) (ensures (v (ulogand #n a b) = v a % pow2 m))
+
+assume val ulogxor_lemma_1: #n:nat -> a:usint n -> b:usint n ->
+  Lemma (requires True) (ensures (v (ulogxor #n a b) = v (ulogxor #n b a)))
+assume val ulogxor_lemma_2: #n:nat -> a:usint n ->
+  Lemma (requires True) (ensures (v (ulogxor #n a (uzero n)) = v a))
+assume val ulogxor_lemma_3: #n:pos -> a:usint n ->
+  Lemma (requires True) (ensures (v (ulogxor #n a (uones n)) = v (ulognot #n a)))
+assume val ulogxor_lemma_4: n:nat -> a:usint n ->
+  Lemma (requires True) (ensures (v (ulogxor #n a a) = 0))
+
+assume val ulogor_lemma_1: #n:nat -> a:usint n -> b:usint n ->
+  Lemma (requires True) (ensures (v (ulogor #n a b) = v (ulogor #n b a)))
+assume val ulogor_lemma_2: #n:nat -> a:usint n ->
+  Lemma (requires True) (ensures (v (ulogor #n a (uzero n)) = v a))
+assume val ulogor_lemma_3: #n:pos -> a:usint n ->
+  Lemma (requires True) (ensures (v (ulogor #n a (uones n)) = v (uones n)))
+
+assume val ulognot_lemma_1: #n:nat -> a:usint n ->
+  Lemma (requires True) (ensures (v (ulognot #n (ulognot #n a)) = v a))
+assume val ulognot_lemma_2: #n:pos ->
+  Lemma (requires True) (ensures (v (ulognot #n (uzero n)) = v (uones n)))
+
+(* Casts *)
+assume val to_usint: m:nat -> a:sint -> Tot (b:usint m{v b = (v a) % pow2 m})
+assume val to_ssint: m:pos -> a:sint -> Tot (b:ssint m{v b = cmod (v a) (pow2 m)})
+
+(* Shift operators *)
+assume val sshift_right: #n:pos -> a:ssint n -> s:nat ->
+  Tot (b:ssint n{v b = div_eucl (v a) (pow2 s)})
+assume val sshift_left: #n:pos -> a:ssint n -> s:nat ->
+  Tot (b:ssint n{v b = cmod ((v a) * pow2 s) (pow2 n)})
+assume val ushift_right: #n:nat -> a:usint n -> s:nat ->
+  Tot (b:usint n{v b = div (v a) (pow2 s)})
+assume val ushift_left: #n:nat -> a:usint n -> s:nat ->
+  Tot (b:usint n{v b = ((v a) * pow2 s) % pow2 n})
+
+val shift_right_logical: #n:pos -> a:ssint n -> s:nat -> Tot (ssint n)
+let shift_right_logical #n a s =
+  to_ssint n (ushift_right #n (to_usint n a) s)
+
+assume val urotate_left: #n:nat -> a:usint n -> s:nat{s <= n} ->
+  Tot (b:usint n{v b = (v a % pow2 (n - s)) * pow2 s + div (v a) (pow2 (n-s))})
+assume val urotate_right: #n:nat -> a:usint n -> s:nat{s <= n} ->
+  Tot (b:usint n{v b = (v a % pow2 s) * pow2 (n-s) + div (v a) (pow2 (s))})
